---
title: 利用求导推导二项式定理
date: 2016-05-26 20:13:54
categories:
- 数学
- 单元微积分
tags:
- 二项式定理

---
设
$$
f(x)=(1+x)^n=a\_0+a\_1x+a\_2x^2+\cdots+a\_nx^n,
$$
下面我们来求$a\_i(1\leq i\leq n)$的表达式.将$f(x)$求导$i$次,可得$f(x)$的$i$阶导数
\begin{equation}\label{eq:1}
f^{(i)}(x)=n(n-1)\cdots(n-i+1)(1+x)^{n-i}=i!a\_i+x\Delta\_{i},
\end{equation}
其中$\Delta\_{i}$是剩下的一堆东西,我们并不关心其具体内容.在式\eqref{eq:1}中,令$x=0$,可得
$$
n(n-1)\cdots (n-i+1)=i! a\_i\Rightarrow
a\_i=\frac{n!}{(n-i)!i!}={n\choose i}.
$$
可见,
$$
(1+x)^n={n\choose 0}+{n\choose 1}x+\cdots+{n\choose
  k}x^{k}+\cdots+{n\choose n}x^n.
$$
所以
$$
(a+b)^n=b^n\left(\frac{a}{b}+1\right)^n={n\choose 0}b^n+{n\choose
  1}ab^{n-1}+\cdots+{n\choose k}a^kb^{n-k}+\cdots+{n\choose n}a^n.
$$